TypeTheory/StlcProp.lean
@@ -15,7 +15,6 @@ theorem canonical_forms_bool :
   | v_false => right; rfl
   | v_abs x T t' => cases ht
 
-count_heartbeats in
 theorem canonical_forms_fun :
     ∀ t T1 T2, (∅ ⊢ t : T1 → T2) → value t →
       ∃ x u, t = <{λ x : T1, u}> := by
@@ -31,7 +30,7 @@ theorem canonical_forms_fun :
 #check step.ST_AppAbs
 
 theorem progress:
-    ∀ t T, (∅ ⊢ t : T) → value t ∨ ∃ t', t -> t' := by
+    ∀ t T, (∅ ⊢ t : T) → value t ∨ ∃ t', t ->- t' := by
   intro t
   induction t with
   | tm_var s => intro T h; contradiction
@@ -46,16 +45,16 @@ theorem progress:
         rcases s1abs with ⟨x, u, rfl⟩
         right
         rcases ih2 with (h2l | ⟨s2', hs2'⟩)
-        · use <{u [x := s2]}>
+        · use u [x := s2]
           apply step.ST_AppAbs
           exact h2l
-        · use <{<{λ x: T1, u}> ↠ s2'}>
+        · use λ x: T1, u ↠ s2'
           apply step.ST_App2
           · exact value.v_abs x T1 u
           assumption
       · right
         rcases hr with ⟨s1', hs1'⟩
-        use <{s1' ↠ s2}>
+        use s1' ↠ s2
         apply step.ST_App1
         · exact hs1'
   | tm_abs x T t _ => exact fun T1 _ => Or.inl (value.v_abs x T t)
@@ -77,6 +76,116 @@ theorem progress:
       · use <{If x' Then t1 Else t2}>
         apply step.ST_If
         exact hx'
+
+open partialmap
+
+count_heartbeats in
+theorem weakening : ∀ Γ Γ' t T,
+    includedin Γ Γ' → (Γ ⊢ t : T) → (Γ' ⊢ t : T) := by
+  intro Γ Γ' t T h ht
+  induction ht generalizing Γ' with
+  | T_Var Γ'' x T1 h1 =>
+    apply has_type.T_Var
+    exact h.property h1
+  | T_Abs Γ'' x T1 T2 t2 _ a_ih =>
+    apply has_type.T_Abs
+    let insertincluded := includedin_insert h x T1
+    exact (a_ih _ insertincluded)
+  | T_app Γ'' t1 t2 T1 T2 _ _ a_iht1 a_iht2 =>
+    refine has_type.T_app ?_ t1 t2 T1 T2 ?_1 ?_2
+    · exact a_iht1 _ h
+    · exact a_iht2 _ h
+  | T_True => exact has_type.T_True _
+  | T_False => exact has_type.T_False _
+  | T_If Γ'' x t2 t3 T _ _ _ a_ihx a_iht2 a_iht3 =>
+    refine has_type.T_If Γ' x t2 t3 T ?_ ?_ ?_3
+    · exact a_ihx _ h
+    · exact a_iht2 _ h
+    · exact a_iht3 _ h
+
+theorem weakening_empty : ∀ Γ t T,
+    (∅ ⊢ t : T) → (Γ ⊢ t : T) := by
+  intro Γ t T ht
+  exact weakening _ _ _ _ (includedin_empty _) ht
+
+theorem substitution_preserves_typing :
+  ∀ Γ x U t v T,
+    (Γ.insert x U ⊢ t : T) →
+    (∅ ⊢ v : U) →
+    (Γ ⊢ t [x := v] : T) := by
+  sorry
+
+theorem preservation :
+  ∀ t t' T,
+    (∅ ⊢ t : T) →
+    t ->- t' →
+    (∅ ⊢ t' : T) := by
+  sorry
+
+theorem preservation' :
+  ∀ t t' T,
+    (∅ ⊢ t : T) →
+    t ->* t' →
+    (∅ ⊢ t' : T) := by
+  intro t t' T ht htt'
+  induction htt' generalizing T with
+  | multi_refl t => exact ht
+  | multi_step x y z rxy syz a_ih =>
+    apply a_ih
+    exact preservation x y T ht rxy
+
+  sorry
+
+theorem not_subject_expansion :
+  ∃ t t' T,
+    t ->- t' ∧ (∅ ⊢ t' : T) ∧ ¬ (∅ ⊢ t : T) := by
+  sorry
+
+def stuck (t : tm) : Prop :=
+  (normal_form step) t ∧ ¬ value t
+
+theorem type_soundness :
+  ∀ t t' T,
+    (∅ ⊢ t : T) → t ->* t' → ¬ stuck t' := by
+  intro t t' T ht multi
+  let ht' : (∅ ⊢ t' : T) := preservation' t t' T ht multi
+  intro ⟨h1, h2⟩
+  rcases (progress t' T ht') with (hl | hr)
+  · exact h2 hl
+  · exact h1 hr
+
+theorem unique_types :
+  ∀ Γ e T T',
+    (Γ ⊢ e : T) → (Γ ⊢ e : T') → T = T' := by
+  sorry
+
+class inductive appears_free_in (x : String) : tm → Prop :=
+  | afi_var : appears_free_in x <{x}>
+  | afi_app1 : ∀ t1 t2, appears_free_in x t1 → appears_free_in x <{t1 ↠ t2}>
+  | afi_app2 : ∀ t1 t2, appears_free_in x t2 → appears_free_in x <{t1 ↠ t2}>
+  | afi_abs : ∀ y T t, x ≠ y → appears_free_in x t → appears_free_in x <{λ y : T, t}>
+  | afi_if1 : ∀ t1 t2 t3, appears_free_in x t1 → appears_free_in x <{If t1 Then t2 Else t3}>
+  | afi_if2 : ∀ t1 t2 t3, appears_free_in x t2 → appears_free_in x <{If t1 Then t2 Else t3}>
+  | afi_if3 : ∀ t1 t2 t3, appears_free_in x t3 → appears_free_in x <{If t1 Then t2 Else t3}>
+
+def closed (t : tm) : Prop :=
+  ∀ x, ¬ appears_free_in x t
+
+theorem free_in_context :
+  ∀ x t T Γ,
+    (appears_free_in x t) → (Γ ⊢ t : T) → (∃ U, Γ.lookup x = some U) := by
+  sorry
+
+theorem typable_empty_closed :
+  ∀ t T,
+    (∅ ⊢ t : T) → closed t := by
+  sorry
+
+theorem context_invariance :
+  ∀ Γ Γ' t T,
+    (Γ ⊢ t : T) → (∀ x, appears_free_in x t → Γ.lookup x = Γ'.lookup x) → (Γ' ⊢ t : T) := by
+  sorry
+
 end STLC
 
 #check Finmap
